correctness

proof/examples/ladder/ladder_correct.ec
@@ -1,76 +1,109 @@
 require import AllCore IntDiv CoreMap List.
 
 
+require import StdOrder.
+import IntOrder.
 
-op ith_bit : int -> int -> bool.
-op parity : int -> int -> bool.
 
-axiom prop1 n x: parity x (n-1)  => ith_bit x (n-1)  => !ith_bit x n.
-axiom prop2 n x: parity x (n-1)  => !ith_bit x (n-1)  => ith_bit x n.
-axiom prop3 n x: !parity x (n - 1)  => ith_bit x (n-1) = ith_bit  x n.
+type bits = bool list.
+
+op ith_bit : bits -> int -> bool.
+op parity : bits -> int -> bool.
+
+op tonat : bits -> int.
+op fromnat : int -> bits.
+
+axiom prop1 n x: parity x (n-1)  => nth witness x (n-1)  => !nth witness x n.
+axiom prop2 n x: parity x (n-1)  => !nth witness x (n-1)  => nth witness x n.
+axiom prop3 n x: !parity x (n - 1)  => nth witness x (n-1) = nth witness x n.
+axiom prop4 : tonat[true] = 1.
+axiom prop5 : tonat[false] = 0.
+
+
+axiom prop6 s :  tonat (true :: s) = 2 * (tonat s) + 1.
+axiom prop7 s :  tonat (false :: s) = 2 * (tonat s).
+axiom prop8 s :  0 <= tonat s  .
 
 
 module M = {
-  
-  proc expm_naive (p:int, x:int, n:int) : int = {
+  (* simple to prove correctness *)
+  proc expm_naive (x:int, n:bits) : int = {
     
     var x1:int;
     var ctr:int;
     var x2:int;
-    var bit:bool;
-    
-    ctr <- 4;
-    x1 <- x;
-    x2 <- x1 * x1; 
-
-    while (0 <= ctr) {
+    var bit:bool;    
+    ctr <- size n;
+    x1 <- 1;
+    x2 <- x; 
+    while (0 < ctr) {
       ctr <- (ctr - 1);
-      (x1,x2) <- (ith_bit n ctr) ? ((x1 * x2), (x2 * x2)) : ((x1*x1),(x1*x2));
+      (x1,x2) <- (nth witness n ctr) ? ((x1*x2), (x2*x2)) : ((x1*x1), (x1*x2));
     }
     return x1;
-  }
-  
+  }  
 
-  proc expm (p:int, x:int, n:int) : int = {
-    
+  (* constant time  *)
+  proc expm (x:int, n:bits) : int = {  
     var x1:int;
     var ctr:int;
     var x2:int;
     var bit:bool;
     
-    ctr <- 4;
-    x1 <- x;
-    x2 <- x1 * x1; 
+    ctr <- size n;
+    x1 <- 1;
+    x2 <- x ; 
 
-    while (0 <= ctr) {
+    while (0 < ctr) {
       ctr <- (ctr - 1);
       (x1,x2) <- if parity n ctr then (x2,x1) else (x1, x2);
       x1 <- x1 * x2;
       x2 <- x2 * x2;
     }
 
-    (x1,x2) <- if ! ith_bit n ctr then (x2,x1) else (x1, x2);    
+    (x1,x2) <- if ! nth witness n ctr then (x2,x1) else (x1, x2);    
     return x1;
     
  } 
-
-  
 }.
 
-
-
+lemma exp_correct xx nn : 
+  hoare[ M.expm_naive : arg = (xx, nn) /\  0 < size nn /\ nth witness nn (size nn) = true ==> res = xx ^ (tonat nn)].
+proof. 
+proc. 
+seq 3 : (ctr = size n /\ x1 = 1 /\ x2 = x /\  0 < size n /\ x = xx /\ n = nn /\ ctr <= size n   ). wp.  skip. progress. 
+while (x1 = x ^ tonat (drop ctr n) /\ x2 = x1 * x /\ ctr <= size n).
+wp. skip.  progress.
+case (nth witness n{hr} (ctr{hr} - 1)). progress.
+  have -> : (drop (ctr{hr} - 1) n{hr}) = true :: (drop (ctr{hr} ) n{hr}).  
+  rewrite (drop_nth witness). progress. smt(). smt().
+  rewrite H1. auto.
+rewrite prop6. 
+pose n := tonat (drop ctr{hr} n{hr}). 
+have ->: x{hr} ^ n * (x{hr} ^ n * x{hr}) 
+  = (x{hr} ^ n * x{hr} ^ n) * x{hr}. smt.
+have -> : x{hr} ^ n * x{hr} ^ n  = x{hr} ^ (2 * n). smt.
+smt.
+progress. 
+have -> : (drop (ctr{hr} - 1) n{hr}) = false :: (drop (ctr{hr} ) n{hr}).  
+rewrite (drop_nth witness). progress. smt(). smt(). rewrite H1.
+auto. rewrite prop7. smt. 
+case (nth witness n{hr} (ctr{hr} - 1)). progress. smt().
+progress. smt().
+smt().
+skip. progress. smt.
+smt.
+qed.
 
 
 lemma exp_eq : 
-  equiv[ M.expm_naive ~ M.expm : ={arg} /\ ith_bit n{1} 4 = true ==> ={res}].
+  equiv[ M.expm_naive ~ M.expm : ={arg} /\ nth witness n{1} (size n{1}) = true ==> ={res}].
 proc.
-seq 3 3 : (={x1,x2,ctr,n} /\ ctr{1} = 4 /\ ith_bit n{1} 4 = true).  wp.  skip.  progress. 
+seq 3 3 : (={x1,x2,ctr,n} /\ ctr{1} = (size n{1}) /\ nth witness n{1} (size n{1}) = true).  wp.  skip.  progress. 
 
-seq 1 1 : (={ctr, n} /\ (ith_bit n{2} ctr{2} => x2{2} = x2{1} /\ x1{2} = x1{1})  /\ ((!ith_bit n{2} ctr{2}) =>  (x1{1} = x2{2} /\ x2{1} = x1{2})) /\ ith_bit n{1} 4 = true).
+seq 1 1 : (={ctr, n} /\ (nth witness n{2} ctr{2} => x2{2} = x2{1} /\ x1{2} = x1{1})  /\ ((!nth witness n{2} ctr{2}) =>  (x1{1} = x2{2} /\ x2{1} = x1{2})) /\ nth witness n{1} (size n{1}) = true).
 
-
-
-while (={ctr, n} /\ (ith_bit n{2} ctr{2} => x2{2} = x2{1} /\ x1{2} = x1{1})  /\ ((!ith_bit n{2} ctr{2}) =>  (x1{1} = x2{2} /\ x2{1} = x1{2}) )).
+while (={ctr, n} /\ (nth witness n{2} ctr{2} => x2{2} = x2{1} /\ x1{2} = x1{1})  /\ ((!nth witness n{2} ctr{2}) =>  (x1{1} = x2{2} /\ x2{1} = x1{2}) )).
 wp. skip. progress.
 rewrite H3. simplify.  
 
